theories/rust_typing/program_rules.v
@@ -22,11 +22,15 @@ Section typing.
 
   Global Instance related_to_named_lfts M : RelatedTo (named_lfts M) | 100 :=
     {| rt_fic := FindNamedLfts |}.
+
   Global Instance related_to_gvar_pobs {rt} γ (r : rt) : RelatedTo (gvar_pobs γ r) | 100 :=
     {| rt_fic := FindGvarPobsP γ |}.
 
   Global Instance related_to_credit_store n m : RelatedTo (credit_store n m) | 100 :=
     {| rt_fic := FindCreditStore |}.
+
+  Global Instance related_to_na_own π E : RelatedTo (na_own π E) | 100 :=
+    {| rt_fic := FindNaOwn π |}.
 
   Global Instance related_to_freeable l n q k : RelatedTo (freeable_nz l n q k) | 100 :=
     {| rt_fic := FindFreeable l |}.
@@ -181,6 +185,23 @@ Section typing.
   Global Instance find_in_context_credit_store_inst :
     FindInContext FindCreditStore FICSyntactic | 1 :=
     λ T, i2p (find_in_context_credit_store T).
+
+  (** NaOwn *)
+  Lemma subsume_na_own π E E' T :
+    ⌜E = E'⌝ ∗ T ⊢ subsume (Σ := Σ) (na_own π E) (na_own π E') T.
+  Proof. iIntros "(-> & $) $". Qed.
+  Global Instance subsume_na_own_inst π E E' : Subsume (na_own π E) (na_own π E') :=
+    λ T, i2p (subsume_na_own π E E' T).
+
+  Lemma find_in_context_na_own π T :
+    (∃ E, na_own π E ∗ T E) ⊢
+    find_in_context (FindNaOwn π) T.
+  Proof.
+    iDestruct 1 as (E) "[Hna HT]". iExists E. by iFrame.
+  Qed.
+  Global Instance find_in_context_na_own_inst π :
+    FindInContext (FindNaOwn π) FICSyntactic | 1 :=
+    λ T, i2p (find_in_context_na_own π T).
 
   (** FindOptLftDead *)
   Lemma subsume_lft_dead κ1 κ2 T :
@@ -1436,11 +1457,11 @@ Section typing.
     ⌜bor_kind_writeable bmin0⌝ ∗ [† κ] ∗ typed_place π E L l (◁ ty) r bmin0 b P T
     ⊢ typed_place π E L l (BlockedLtype ty κ) r bmin0 b P T.
   Proof.
-    iIntros "(%Hw & Hdead & Hp)". iIntros (????) "#(LFT & TIME & LLCTX) #HE HL Hna Hincl0 Hl HΦ".
+    iIntros "(%Hw & Hdead & Hp)". iIntros (????) "#(LFT & TIME & LLCTX) #HE HL Hincl0 Hl HΦ".
     iApply fupd_place_to_wp.
     iMod (unblock_blocked with "Hdead Hl") as "Hl"; first done.
     iModIntro.
-    iApply ("Hp" with "[//] [//] [$LFT $TIME $LLCTX] HE HL Hna Hincl0 Hl").
+    iApply ("Hp" with "[//] [//] [$LFT $TIME $LLCTX] HE HL Hincl0 Hl").
     iIntros (L' κs l2 b2 bmin rti tyli ri strong weak) "Hincl1 Hl2 Hs HT HL".
     iApply ("HΦ" $! _ _ _ _ _ _ _ _ _ _ with "Hincl1 Hl2 [Hs] HT HL").
     iSplit.
@@ -1464,11 +1485,11 @@ Section typing.
     ⌜bor_kind_writeable bmin0⌝ ∗ [† κ] ∗ typed_place π E L l (◁ ty) r bmin0 b P T
     ⊢ typed_place π E L l (ShrBlockedLtype ty κ) r bmin0 b P T.
   Proof.
-    iIntros "(%Hw & Hdead & Hp)". iIntros (????) "#(LFT & TIME & LLCTX) #HE HL Hna Hincl0 Hl HΦ".
+    iIntros "(%Hw & Hdead & Hp)". iIntros (????) "#(LFT & TIME & LLCTX) #HE HL Hincl0 Hl HΦ".
     iApply fupd_place_to_wp.
     iMod (unblock_shrblocked with "Hdead Hl") as "Hl"; first done.
     iModIntro.
-    iApply ("Hp" with "[//] [//] [$LFT $TIME $LLCTX] HE HL Hna Hincl0 Hl").
+    iApply ("Hp" with "[//] [//] [$LFT $TIME $LLCTX] HE HL Hincl0 Hl").
     iIntros (L' κs l2 b2 bmin rti tyli ri strong weak) "Hincl1 Hl2 Hs HT HL".
     iApply ("HΦ" $! _ _ _ _ _ _ _ _ _ _ with "Hincl1 Hl2 [Hs] HT HL").
     iSplit.
@@ -1492,11 +1513,11 @@ Section typing.
     ⌜bor_kind_writeable bmin0⌝ ∗ lft_dead_list κs ∗ typed_place π E L l (ltype_core lt) r bmin0 b P T
     ⊢ typed_place π E L l (CoreableLtype κs lt) r bmin0 b P T.
   Proof.
-    iIntros "(%Hw & Hdead & Hp)". iIntros (????) "#(LFT & TIME & LLCTX) #HE HL Hna Hincl0 Hl HΦ".
+    iIntros "(%Hw & Hdead & Hp)". iIntros (????) "#(LFT & TIME & LLCTX) #HE HL Hincl0 Hl HΦ".
     iApply fupd_place_to_wp.
     iMod (unblock_coreable with "Hdead Hl") as "Hl"; first done.
     iModIntro.
-    iApply ("Hp" with "[//] [//] [$LFT $TIME $LLCTX] HE HL Hna Hincl0 Hl").
+    iApply ("Hp" with "[//] [//] [$LFT $TIME $LLCTX] HE HL Hincl0 Hl").
     iIntros (L' κs' l2 b2 bmin rti tyli ri strong weak) "Hincl1 Hl2 Hs HT HL".
     iApply ("HΦ" $! _ _ _ _ _ _ _ _ _ _ with "Hincl1 Hl2 [Hs] HT HL").
     iSplit.
@@ -1523,12 +1544,12 @@ Section typing.
       introduce_with_hooks E L' R (λ L'', typed_place π E L'' l lt r bmin0 b P T))
     ⊢ typed_place π E L l lt (PlaceGhost γ) bmin0 b P T.
   Proof.
-    iIntros "(% & %Hw & Hres)". iIntros (????) "#CTX #HE HL Hna Hincl0 Hl HΦ".
+    iIntros "(% & %Hw & Hres)". iIntros (????) "#CTX #HE HL Hincl0 Hl HΦ".
     iApply fupd_place_to_wp.
     iMod ("Hres" with "[] [] CTX HE HL Hl") as "(%L' & %r & %R & %prog & Hstep & HL & HP)"; [done.. | ].
     iMod "Hstep" as "(Hl & HR)".
     iMod ("HP" with "[] HE HL HR") as "(%L'' & HL & HP)"; first done.
-    iModIntro. iApply ("HP" with "[//] [//] CTX HE HL Hna Hincl0 Hl").
+    iModIntro. iApply ("HP" with "[//] [//] CTX HE HL Hincl0 Hl").
     iIntros (L1 κs l2 b2 bmin rti tyli ri strong weak) "Hincl1 Hl2 Hs HT HL".
     iApply ("HΦ" $! _ _ _ _ _ _ _ _ _ _ with "Hincl1 Hl2 [Hs] HT HL").
     iSplit.
@@ -1578,7 +1599,7 @@ Section typing.
     typed_place π E L l (◁ ty) (PlaceIn r) bmin0 (Owned wl) (DerefPCtx Na1Ord PtrOp true :: P) T.
   Proof.
     iIntros (Hot) "HT".
-    iIntros (????) "#CTX #HE HL Hna #Hincl Hl Hcont". iApply fupd_place_to_wp.
+    iIntros (????) "#CTX #HE HL #Hincl Hl Hcont". iApply fupd_place_to_wp.
     iPoseProof (ofty_ltype_acc_owned ⊤ with "Hl") as "(%ly & %Halg & %Hly & Hsc & Hlb & >(%v & Hl & Hv & Hcl))"; first done.
     simpl. iModIntro.
     iDestruct "CTX" as "(LFT & TIME & LLCTX)".
@@ -1593,7 +1614,7 @@ Section typing.
     iMod ("Ha" with "Hl [//] Hsc Hv") as "Hl".
     iModIntro.
     iExists l2. rewrite mem_cast_id_loc. iSplitR; first done.
-    iApply ("HT" with "[//] [//] [$LFT $TIME $LLCTX] HE HL Hna [] Hl2").
+    iApply ("HT" with "[//] [//] [$LFT $TIME $LLCTX] HE HL [] Hl2").
     { iApply bor_kind_incl_refl. }
     iIntros (L2 κs l3 b3 bmin rti ltyi ri strong weak) "#Hincl1 Hl3 Hcl HT HL".
     iApply ("Hcont" with "[//] Hl3 [Hcl Hl] HT HL").
@@ -1640,7 +1661,7 @@ Section typing.
     ⊢ typed_place π E L l (◁ ty) (PlaceIn r) bmin0 (Uniq κ γ) (DerefPCtx Na1Ord PtrOp true :: P) T.
   Proof.
     iIntros (Hot) "(%Hal & HT)".
-    iIntros (????) "#CTX #HE HL Hna #Hincl Hl Hcont". iApply fupd_place_to_wp.
+    iIntros (????) "#CTX #HE HL #Hincl Hl Hcont". iApply fupd_place_to_wp.
     iPoseProof (llctx_interp_acc_noend with "HL") as "(HL & HL_cl)".
     iMod (fupd_mask_subseteq lftE) as "HF_cl"; first done.
     iMod (Hal with "HE HL") as "(%q' & Htok & HL_cl2)"; first done.
@@ -1660,7 +1681,7 @@ Section typing.
     iPoseProof ("HL_cl" with "HL") as "HL".
     iModIntro.
     iExists l2. rewrite mem_cast_id_loc. iSplitR; first done.
-    iApply ("HT" with "[//] [//] [$LFT $TIME $LLCTX] HE HL Hna [] Hl2").
+    iApply ("HT" with "[//] [//] [$LFT $TIME $LLCTX] HE HL [] Hl2").
     { iApply bor_kind_incl_refl. }
     iIntros (L2 κs l3 b3 bmin rti ltyi ri strong weak) "#Hincl1 Hl3 Hcl HT HL".
     iApply ("Hcont" with "[//] Hl3 [Hcl Hl] HT HL").
@@ -1697,7 +1718,7 @@ Section typing.
     ⊢ typed_place π E L l (◁ ty) (PlaceIn r) bmin0 (Shared κ) (DerefPCtx Na1Ord PtrOp true :: P) T.
   Proof.
     iIntros (Hot) "(%Hal & HT)".
-    iIntros (????) "#CTX #HE HL Hna #Hincl #Hl Hcont". iApply fupd_place_to_wp.
+    iIntros (????) "#CTX #HE HL #Hincl #Hl Hcont". iApply fupd_place_to_wp.
     iPoseProof (llctx_interp_acc_noend with "HL") as "(HL & HL_cl)".
     iMod (Hal with "HE HL") as "(%q' & Htok & HL_cl2)"; first done.
     iPoseProof (ofty_ltype_acc_shared ⊤ with "Hl") as "(%ly & %Halg & %Hly & Hlb & >Hb)"; first done.
@@ -1719,7 +1740,7 @@ Section typing.
     iMod ("HL_cl2" with "Htok") as "HL". iPoseProof ("HL_cl" with "HL") as "HL".
     iModIntro.
     iExists l2. rewrite mem_cast_id_loc. iSplitR; first done.
-    iApply ("HT" with "[//] [//] [$LFT $TIME $LLCTX] HE HL Hna [] Hl2").
+    iApply ("HT" with "[//] [//] [$LFT $TIME $LLCTX] HE HL [] Hl2").
     { iApply bor_kind_incl_refl. }
     iIntros (L2 κs l3 b3 bmin rti ltyi ri strong weak) "#Hincl1 Hl3 Hcl HT HL".
     iApply ("Hcont" with "[//] Hl3 [Hcl Hv] HT HL").
@@ -1750,9 +1771,9 @@ Section typing.
         None)
     ⊢ typed_place π E L l (OpenedLtype lt_cur lt_inner lt_full Cpre Cpost) r bmin0 (Owned wl) P T.
   Proof.
-    iIntros "HT". iIntros (Φ F ??) "#CTX #HE HL Hna #Hincl0 Hl HR".
+    iIntros "HT". iIntros (Φ F ??) "#CTX #HE HL #Hincl0 Hl HR".
     iPoseProof (opened_ltype_acc_owned with "Hl") as "(Hl & Hcl)".
-    iApply ("HT" with "[//] [//] CTX HE HL Hna [] Hl").
+    iApply ("HT" with "[//] [//] CTX HE HL [] Hl").
     { destruct bmin0; done. }
     iIntros (L' ??????? strong weak) "? Hl Hv".
     iApply ("HR" with "[$] Hl").
@@ -1779,9 +1800,9 @@ Section typing.
         None)
     ⊢ typed_place π E L l (OpenedLtype lt_cur lt_inner lt_full Cpre Cpost) r bmin0 (Uniq κ γ) P T.
   Proof.
-    iIntros "HT". iIntros (Φ F ??) "#CTX #HE HL Hna #Hincl0 Hl HR".
+    iIntros "HT". iIntros (Φ F ??) "#CTX #HE HL #Hincl0 Hl HR".
     iPoseProof (opened_ltype_acc_uniq with "Hl") as "(Hl & Hcl)".
-    iApply ("HT" with "[//] [//] CTX HE HL Hna [] Hl").
+    iApply ("HT" with "[//] [//] CTX HE HL [] Hl").
     { destruct bmin0; done. }
     iIntros (L' ??????? strong weak) "? Hl Hv".
     iApply ("HR" with "[$] Hl").
@@ -1808,10 +1829,10 @@ Section typing.
     ⊢ typed_place π E L l (ShadowedLtype lt_cur (#r_cur) lt_full) r_full bmin0 (Shared κ) P T.
   Proof.
     iIntros "(Houtl & HT)".
-    iIntros (????) "#CTX #HE HL Hna Hincl Hl Hc".
+    iIntros (????) "#CTX #HE HL Hincl Hl Hc".
     iPoseProof (lctx_bor_kind_outlives_all_use with "Houtl HE HL") as "#Houtl'".
     iPoseProof (shadowed_ltype_acc_cur with "Hl") as "(Hcur & Hcl)".
-    iApply ("HT" with "[//] [//] CTX HE HL Hna Hincl Hcur").
+    iApply ("HT" with "[//] [//] CTX HE HL Hincl Hcur").
     iIntros (L' κs l2 b2 bmin rti ltyi ri strong weak) "Hincl' Hl Hcc".
     iApply ("Hc" with "Hincl' Hl").
     iSplit; simpl.
@@ -2110,7 +2131,7 @@ Section typing.
 
   Import EqNotations.
   (** Entry point for checking reads *)
-  Lemma type_read π E L T T' e ot : (* TODO: MagicType *)
+  Lemma type_read π E L T T' e ot :
     (** Decompose the expression *)
     IntoPlaceCtx π E e T' →
     T' L (λ L' K l,
@@ -2135,8 +2156,7 @@ Section typing.
     iIntros (HT') "HT'". iIntros (Φ F ???) "#CTX #HE HL Hna HΦ".
     iApply (HT' with "CTX HE HL Hna HT'").
     iIntros (L' K l) "HL Hna". iDestruct 1 as ([rt ([ty r] & ?)]) "[Hl HP]".
-    iApply ("HP" with "[//] [//] CTX HE HL [] [] Hl").
-    { admit. }
+    iApply ("HP" with "[//] [//] CTX HE HL [] Hl").
     { iApply bor_kind_incl_refl. }
     iIntros (L'' κs l2 b2 bmin rti tyli ri strong weak) "#Hincl1 Hl2 Hs HT HL".
     iApply "HΦ".
@@ -2188,7 +2208,7 @@ Section typing.
       cbn. iDestruct ("Hfin" with "Hl HR'") as "Hfin".
       iMod ("Hfin" with "[] HE HL HR") as "(%L4 & HL & HT)"; first done.
       iModIntro. iExists _, _, _, _. iFrame.
-  Admitted.
+  Qed.
 
   (** [type_read_end] instance that does a copy *)
   Lemma type_read_ofty_copy E L {rt} π (T : typed_read_end_cont_t rt) b2 bmin br l (ty : type rt) r ot `{!Copyable ty}:
@@ -2318,7 +2338,7 @@ Section typing.
       (this would be required for full generality, because shr_blocked can be below them)
    *)
 
-  Lemma type_write E L T T' e ot v rt (ty : type rt) r π : (* TODO: MagicType *)
+  Lemma type_write E L T T' e ot v rt (ty : type rt) r π :
     IntoPlaceCtx π E e T' →
     T' L (λ L' K l, find_in_context (FindLoc l π) (λ '(existT rto (lt1, r1, b)),
       typed_place π E L' l lt1 r1 b b K (λ (L1 : llctx) (κs : list lft) (l2 : loc) (b2 bmin : bor_kind) rti (lt2 : ltype rti) (ri2 : place_rfn rti) (strong : option $ strong_ctx rti) (weak : option $ weak_ctx rto rti),
@@ -2335,8 +2355,7 @@ Section typing.
     iIntros (HT') "HT'". iIntros (Φ F ???) "#CTX #HE HL Hna HΦ".
     iApply (HT' with "CTX HE HL Hna HT'").
     iIntros (L' K l) "HL Hna". iDestruct 1 as ([rt1 ([ty1 r1] & ?)]) "[Hl HP]".
-    iApply ("HP" with "[//] [//] CTX HE HL [] [] Hl").
-    { admit. }
+    iApply ("HP" with "[//] [//] CTX HE HL [] Hl").
     { iApply bor_kind_incl_refl. }
     iIntros (L'' κs l2 b2 bmin rti tyli ri strong weak) "#Hincl1 Hl2 Hs HT HL".
     iApply ("HΦ"). iIntros "Hv".
@@ -2376,7 +2395,7 @@ Section typing.
         iPoseProof ("Hfin" with "Hl HR'") as "Hfin".
         iMod ("Hfin" with "[//] HE HL HR") as "(%L4 & HL & HT)".
         iModIntro. iExists _. iFrame.
-  Admitted.
+  Qed.
 
   (* TODO: generalize to other places where we can overwrite, but which can't be folded to an ofty *)
 
@@ -2578,7 +2597,7 @@ Section typing.
     Of course, with nested products, this gets more complicated...
    *)
 
-  Lemma type_addr_of_mut π E L (e : expr) (T : typed_addr_of_mut_cont_t) T' : (* TODO: MagicType *)
+  Lemma type_addr_of_mut π E L (e : expr) (T : typed_addr_of_mut_cont_t) T' :
     IntoPlaceCtx π E e T' →
     T' L (λ L1 K l, find_in_context (FindLoc l π) (λ '(existT rto (lt1, r1, b)),
       (* place *)
@@ -2593,8 +2612,7 @@ Section typing.
     iIntros (HT') "HT'". iIntros (Φ F ???) "#CTX #HE HL Hna HΦ".
     iApply (HT' with "CTX HE HL Hna HT'").
     iIntros (L1 K l) "HL Hna". iDestruct 1 as ([rto [[lt1 r1] b]]) "(Hl & Hplace)" => /=.
-    iApply ("Hplace" with "[//] [//] CTX HE HL [] [] Hl").
-    { admit. }
+    iApply ("Hplace" with "[//] [//] CTX HE HL [] Hl").
     { iApply bor_kind_incl_refl. }
     iIntros (L2 κs l2 b2 bmin rti ltyi ri strong weak) "#Hincl Hl2 Hs Hcont HL".
     iApply "HΦ".
@@ -2615,11 +2633,11 @@ Section typing.
 
     iExists L4, _, tyb, rb. iFrame.
     by iApply "HT".
-  Admitted.
+  Qed.
   (* NOTE: instances for [typed_addr_of_mut_end] are in alias_ptr.v *)
 
   (** Top-level rule for creating a mutable borrow *)
-  Lemma type_borrow_mut E L T T' e κ π (orty : option rust_type) : (* TODO: MagicType *)
+  Lemma type_borrow_mut E L T T' e κ π (orty : option rust_type) :
     (** Decompose the expression *)
     IntoPlaceCtx π E e T' →
     T' L (λ L1 K l,
@@ -2661,8 +2679,7 @@ Section typing.
     iIntros (HT') "HT'". iIntros (Φ F ???) "#CTX #HE HL Hna HΦ".
     iApply (HT' with "CTX HE HL Hna HT'").
     iIntros (L1 K l) "HL Hna". iDestruct 1 as ([rt1 ([ty1 r1] & ?)]) "[Hl HP]".
-    iApply ("HP" $! _ F with "[//] [//] CTX HE HL [] [] Hl").
-    { admit. }
+    iApply ("HP" $! _ F with "[//] [//] CTX HE HL [] Hl").
     { iApply bor_kind_incl_refl. }
     iIntros (L2 κs l2 b2 bmin rti tyli ri strong weak) "#Hincl1 Hl2 Hs HT HL2".
     iDestruct "HT" as ([n m]) "(Hstore & HT)".
@@ -2744,7 +2761,7 @@ Section typing.
       iMod ("HT" with "[//] HE HL HR") as "(%L4 & HL & HT)".
       iModIntro. iExists L4, _, _, _, γ, ly. iFrame.
       iSplitR; done.
-  Admitted.
+  Qed.
 
   (** Finish a mutable borrow *)
   Lemma type_borrow_mut_end E L π κ l (rt : Type) (ty : type rt) (r : place_rfn rt) b2 bmin T:
@@ -2855,7 +2872,7 @@ Section typing.
     TypedBorrowMutEnd π E L κ l ty (r) b2 bmin | 20 :=
     λ T, i2p (type_borrow_mut_end E L π κ l rt ty r b2 bmin T).
 
-  Lemma type_borrow_shr E L T T' e κ orty π : (* TODO: MagicType *)
+  Lemma type_borrow_shr E L T T' e κ orty π :
     IntoPlaceCtx π E e T' →
     T' L (λ L1 K l, find_in_context (FindLoc l π) (λ '(existT rto (lt1, r1, b)),
       (* place *)
@@ -2887,8 +2904,7 @@ Section typing.
     iIntros (HT') "HT'". iIntros (Φ F ???) "#CTX #HE HL Hna HΦ".
     iApply (HT' with "CTX HE HL Hna HT'").
     iIntros (L1 K l) "HL Hna". iDestruct 1 as ([rt1 ([ty1 r1] & ?)]) "[Hl HP]".
-    iApply ("HP" $! _ F with "[//] [//] CTX HE HL [] [] Hl").
-    { admit. }
+    iApply ("HP" $! _ F with "[//] [//] CTX HE HL [] Hl").
     { iApply bor_kind_incl_refl. }
     iIntros (L2 κs l2 b2 bmin rti tyli ri strong weak) "#Hincl1 Hl2 Hs HT HL".
     (* bring the place type in the right shape *)
@@ -2967,7 +2983,7 @@ Section typing.
       iMod ("HT" with "[//] HE HL HR") as "(%L4 & HL & HT)".
       iModIntro. iExists L4, _, _, _, _, ly. iFrame.
       iSplitR; done.
-  Admitted.
+  Qed.
 
   Lemma type_borrow_shr_end_owned E L π κ l {rt : Type} (ty : type rt) (r : place_rfn rt) bmin wl T:
     ⌜lctx_bor_kind_incl E L (Uniq κ inhabitant) bmin⌝ ∗
