theories/rust_typing/references.v
@@ -950,7 +950,7 @@ Section rules.
   Proof.
     iIntros "HR" (Φ F ??).
     rewrite /li_tactic /lctx_lft_alive_count_goal.
-    iIntros "#(LFT & TIME & LLCTX) #HE HL Hna Hincl0 HP HΦ/=".
+    iIntros "#(LFT & TIME & LLCTX) #HE HL Hincl0 HP HΦ/=".
     iPoseProof (mut_ltype_acc_owned F with "[$LFT $TIME $LLCTX] HP") as "(%Hly & Hlb & Hb)"; [done.. | ].
     iApply fupd_wp. iMod (fupd_mask_subseteq F) as "HclF"; first done.
     iMod "Hb" as "(%l' & Hl & Hb & Hcl)". iMod "HclF" as "_". iModIntro.
@@ -959,7 +959,7 @@ Section rules.
     iNext. iIntros (st) "Hl Hcred Hc". iMod (fupd_mask_subseteq F) as "HclF"; first done.
     iMod "HclF" as "_". iExists l'.
     iSplitR. { iPureIntro. unfold mem_cast. rewrite val_to_of_loc. done. }
-    iApply ("HR" with "[//] [//] [$LFT $TIME $LLCTX] HE HL Hna [] Hb"). { iApply bor_kind_min_incl_l. }
+    iApply ("HR" with "[//] [//] [$LFT $TIME $LLCTX] HE HL [] Hb"). { iApply bor_kind_min_incl_l. }
     iModIntro. iIntros (L' κs l2 b2 bmin rti tyli ri strong weak) "#Hincl1 Hb Hs".
     iApply ("HΦ" $! _ _ _ _ bmin _ _ _ _ _ with "Hincl1 Hb").
     simpl. iSplit.
@@ -1002,7 +1002,7 @@ Section rules.
   Proof.
     rewrite /lctx_lft_alive_count_goal.
     iIntros "(%κs & %L2 & %Hal & HT)".
-    iIntros (Φ F ??). iIntros "#(LFT & TIME & LLCTX) #HE HL Hna #Hincl0 HP HΦ/=".
+    iIntros (Φ F ??). iIntros "#(LFT & TIME & LLCTX) #HE HL #Hincl0 HP HΦ/=".
     (* get a token *)
     iApply fupd_wp. iMod (fupd_mask_subseteq lftE) as "HclF"; first done.
     iMod (lctx_lft_alive_count_tok lftE with "HE HL") as (q) "(Hκ' & Hclκ' & HL)"; [done.. | ].
@@ -1015,7 +1015,7 @@ Section rules.
     iIntros (st) "Hl Hcred Hcl".
     iExists l'.
     iSplitR. { iPureIntro. unfold mem_cast. rewrite val_to_of_loc. done. }
-    iApply ("HT" with "[//] [//] [$LFT $TIME $LLCTX] HE HL Hna [] Hb"). { iApply bor_kind_min_incl_l. }
+    iApply ("HT" with "[//] [//] [$LFT $TIME $LLCTX] HE HL [] Hb"). { iApply bor_kind_min_incl_l. }
     iModIntro. iIntros (L'' κs' l2 b2 bmin rti tyli ri strong weak) "#Hincl1 Hb Hs".
     iApply ("HΦ" $! _ _ _ _ (Uniq κ' γ' ⊓ₖ bmin) _ _ _ _ _ with "[Hincl1] Hb").
     { iApply bor_kind_incl_trans; last iApply "Hincl1". iApply bor_kind_min_incl_r. }
@@ -1064,7 +1064,7 @@ Section rules.
   Proof.
     rewrite /lctx_lft_alive_count_goal.
     iIntros "(%κs & %L2 & %Hal & HT)".
-    iIntros (Φ F ??). iIntros "#(LFT & TIME & LLCTX) #HE HL Hna #Hincl0 HP HΦ/=".
+    iIntros (Φ F ??). iIntros "#(LFT & TIME & LLCTX) #HE HL #Hincl0 HP HΦ/=".
     (* get a token *)
     iApply fupd_wp. iMod (fupd_mask_subseteq lftE) as "HclF"; first done.
     iMod (lctx_lft_alive_count_tok lftE with "HE HL") as (q) "(Hκ' & Hclκ' & HL)"; [done.. | ].
@@ -1076,7 +1076,7 @@ Section rules.
     iIntros (st) "Hl Hcred". iMod (fupd_mask_mono with "Hb") as "#Hb"; first done.
     iExists l'.
     iSplitR. { iPureIntro. unfold mem_cast. rewrite val_to_of_loc. done. }
-    iApply ("HT" with "[//] [//] [$LFT $TIME $LLCTX] HE HL Hna [] Hb"). { iApply bor_kind_min_incl_l. }
+    iApply ("HT" with "[//] [//] [$LFT $TIME $LLCTX] HE HL [] Hb"). { iApply bor_kind_min_incl_l. }
     iModIntro. iIntros (L'' κs' l2 b2 bmin rti tyli ri strong weak) "#Hincl1 Hb' Hs".
     iApply ("HΦ" $! _ _ _ _ (Shared κ' ⊓ₖ bmin) _ _ _ _ _ with "[Hincl1] Hb'").
     { iApply bor_kind_incl_trans; last iApply "Hincl1". iApply bor_kind_min_incl_r. }
@@ -2512,7 +2512,7 @@ Section rules.
     ⊢ typed_place π E L l (ShrLtype lt2 κ) (#r) bmin0 (Owned wl) (DerefPCtx Na1Ord PtrOp true :: P) T.
   Proof.
     iIntros "HR" (Φ F ??).
-    iIntros "#(LFT & TIME & LLCTX) #HE HL Hna Hincl0 HP HΦ/=".
+    iIntros "#(LFT & TIME & LLCTX) #HE HL Hincl0 HP HΦ/=".
     iPoseProof (shr_ltype_acc_owned F with "[$LFT $TIME $LLCTX] HP") as "(%Hly & Hlb & Hb)"; [done.. | ].
     iApply fupd_wp. iMod (fupd_mask_subseteq F) as "HclF"; first done.
     iMod "Hb" as "(%l' & Hl & Hb & Hcl)". iMod "HclF" as "_". iModIntro.
@@ -2521,7 +2521,7 @@ Section rules.
     iNext. iIntros (st) "Hl Hcred Hc". iMod (fupd_mask_subseteq F) as "HclF"; first done.
     iMod "HclF" as "_". iExists l'.
     iSplitR. { iPureIntro. unfold mem_cast. rewrite val_to_of_loc. done. }
-    iApply ("HR" with "[//] [//] [$LFT $TIME $LLCTX] HE HL Hna [] Hb"). { iApply bor_kind_min_incl_l. }
+    iApply ("HR" with "[//] [//] [$LFT $TIME $LLCTX] HE HL [] Hb"). { iApply bor_kind_min_incl_l. }
     iModIntro. iIntros (L' κs l2 b2 bmin rti tyli ri strong weak) "#Hincl1 Hb Hs".
     iApply ("HΦ" $! _ _ _ _ bmin _ _ _ _ _ with "Hincl1 Hb").
     simpl. iSplit.
@@ -2572,7 +2572,7 @@ Section rules.
   Proof.
     rewrite /lctx_lft_alive_count_goal.
     iIntros "(%κs & %L2 & %Hal & HT)".
-    iIntros (Φ F ??). iIntros "#(LFT & TIME & LLCTX) #HE HL Hna #Hincl0 HP HΦ/=".
+    iIntros (Φ F ??). iIntros "#(LFT & TIME & LLCTX) #HE HL #Hincl0 HP HΦ/=".
     (* get a token *)
     iApply fupd_wp. iMod (fupd_mask_subseteq lftE) as "HclF"; first done.
     iMod (lctx_lft_alive_count_tok lftE with "HE HL") as (q) "(Hκ' & Hclκ' & HL)"; [done.. | ].
@@ -2584,7 +2584,7 @@ Section rules.
     iNext. iIntros (st) "Hl Hcred Hc". iMod (fupd_mask_subseteq F) as "HclF"; first done.
     iMod "HclF" as "_". iExists l'.
     iSplitR. { iPureIntro. unfold mem_cast. rewrite val_to_of_loc. done. }
-    iApply ("HT" with "[//] [//] [$LFT $TIME $LLCTX] HE HL Hna [] Hb"). { iApply bor_kind_incl_refl. }
+    iApply ("HT" with "[//] [//] [$LFT $TIME $LLCTX] HE HL [] Hb"). { iApply bor_kind_incl_refl. }
     iModIntro. iIntros (L' κs' l2 b2 bmin rti tyli ri strong weak) "#Hincl1 Hb Hs".
     iApply ("HΦ" $! _ _ _ _ bmin _ _ _ _ _ with "Hincl1 Hb").
     simpl. iSplit.
@@ -2635,7 +2635,7 @@ Section rules.
   Proof.
     rewrite /lctx_lft_alive_count_goal.
     iIntros "(%κs & %L2 & %Hal & HT)".
-    iIntros (Φ F ??). iIntros "#(LFT & TIME & LLCTX) #HE HL Hna #Hincl0 HP HΦ/=".
+    iIntros (Φ F ??). iIntros "#(LFT & TIME & LLCTX) #HE HL #Hincl0 HP HΦ/=".
     (* get a token *)
     iApply fupd_wp. iMod (fupd_mask_subseteq lftE) as "HclF"; first done.
     iMod (lctx_lft_alive_count_tok lftE with "HE HL") as (q) "(Hκ' & Hclκ' & HL)"; [done.. | ].
@@ -2647,7 +2647,7 @@ Section rules.
     iIntros (st) "Hl Hcred". iMod (fupd_mask_mono with "Hb") as "#Hb"; first done.
     iExists l'.
     iSplitR. { iPureIntro. unfold mem_cast. rewrite val_to_of_loc. done. }
-    iApply ("HT" with "[//] [//] [$LFT $TIME $LLCTX] HE HL Hna [] Hb"). { iApply bor_kind_min_incl_l. }
+    iApply ("HT" with "[//] [//] [$LFT $TIME $LLCTX] HE HL [] Hb"). { iApply bor_kind_min_incl_l. }
     iModIntro. iIntros (L'' κs' l2 b2 bmin rti tyli ri strong weak) "#Hincl1 Hb' Hs".
     iApply ("HΦ" $! _ _ _ _ (Shared κ' ⊓ₖ bmin) _ _ _ _ _ with "[Hincl1] Hb'").
     { iApply bor_kind_incl_trans; last iApply "Hincl1". iApply bor_kind_min_incl_r. }
